Declarative/Properties.v
@@ -1,174 +1,137 @@
 Require Import Declarative.BasicProperties.
 Require Import Declarative.KindReasoning.
+Require Import Declarative.OccurenceReasoning.
+
+Require Import Program.Tactics.
+
+Lemma binds_subst : forall Γ1 Γ2 x x' A B e,
+    ⊢ Γ1, x' : B,, Γ2 ->
+    x : A ∈ Γ1, x' : B,, Γ2 -> x <> x' -> x : [e / x'] A ∈ Γ1 ,, [e // x'] Γ2.
+Proof.
+  induction Γ2; simpl; intros.
+  - destruct H0.
+    + inversion H0. subst. contradiction.
+    + inversion H. subst.
+      assert (x' # A) by (eapply notin_dom_bind_fresh; eauto).
+      rewrite fresh_subst_eq; auto.
+  - destruct a. destruct H0.
+    + inversion H0. subst. auto.
+    + right. inversion H. apply IHΓ2 with B; auto.
+Qed.
+
+Lemma subst_ctx_distr_cons : forall Γ x A y e,
+    [e // y] Γ , x : [e / y] A = [e // y] (Γ , x : A).
+Proof.
+  intros. reflexivity.
+Qed.
+
+Lemma dom_subst_equal : forall Γ x v,
+    dom ([v // x] Γ) = dom Γ.
+Proof.
+  induction Γ; intros.
+  + reflexivity.
+  + destruct a. simpl. now rewrite (IHΓ x v).
+Qed.
+
+Import AtomSetProperties.
+
+Lemma dom_insert_subset : forall Γ2 Γ1 a (A : expr),
+    union (dom Γ2) (dom Γ1) [<=] dom (Γ1 , a : A ,, Γ2).
+Proof.
+  induction Γ2; simpl; intros.
+  - apply subset_add_2. intro. intros.
+    now apply empty_union_1 in H.
+  - destruct a. intro. intros.
+    apply union_add in H.
+    assert (add a (union (dom Γ2) (dom Γ1)) [<=] add a (dom (Γ1 , a0 : A ,, Γ2))).
+    + apply subset_add_3. auto.
+      apply subset_add_2. apply IHΓ2.
+    + now apply H0.
+Qed.
+
+Theorem substitution : forall Γ1 Γ2 x A B e1 e2 e3,
+  Γ1 , x : B ,, Γ2 ⊢ e1 <: e2 : A ->
+  Γ1 ⊢ e3 : B -> mono_type e3 ->
+  Γ1 ,, [e3 // x] Γ2 ⊢ [e3 / x] e1 <: [e3 / x] e2 : [e3 / x] A.
+Proof.
+  intros until e3. intros Hsub Hsub3 Mono.
+  remember (Γ1 , x : B ,, Γ2) as Γ.
+  generalize dependent HeqΓ.
+  generalize x Γ2. clear x Γ2.
+  apply sub_mut with
+      (P := fun Γ e1 e2 A => fun (_ : Γ ⊢ e1 <: e2 : A) =>
+         forall x Γ2, Γ = Γ1, x : B,, Γ2 ->
+         Γ1 ,, [e3 // x] Γ2 ⊢ [e3 / x] e1 <: [e3 / x] e2 : [e3 / x] A)
+      (P0 := fun Γ => fun (_ : ⊢ Γ) =>
+         forall x Γ2, Γ = Γ1 , x : B,, Γ2 -> ⊢ Γ1 ,, [e3 // x] Γ2);
+      simpl; intros; subst.
+  - destruct (x == x0).
+    + subst. assert (A0 = B) by (eapply binds_type_equal; eauto). subst.
+      rewrite fresh_subst_eq. apply weakening_app; auto.
+      apply prefix_wf in w. inversion w. subst.
+      eapply fresh_ctx_fresh_expr; eauto.
+    + apply s_var. auto.
+      apply binds_subst with B; auto.
+  - auto.
+  - auto.
+  - auto.
+  - apply s_abs with (add x L) k.
+    + auto.
+    + intros. distribute_ctx. rewrite subst_ctx_distr_cons.
+      repeat rewrite subst_open_var_assoc; auto 2.
+  - apply s_pi with (add x L) k1.
+    + auto.
+    + auto.
+    + auto.
+    + intros. distribute_ctx. rewrite subst_ctx_distr_cons.
+      repeat rewrite subst_open_var_assoc; auto 2.
+    + intros. distribute_ctx. rewrite subst_ctx_distr_cons.
+      repeat rewrite subst_open_var_assoc; auto 2.
+  - rewrite subst_open_distr; auto.
+    apply s_app with ([e3 / x] A0); auto.
+  - apply s_forall with (add x L) k.
+    + auto.
+    + intros. distribute_ctx. rewrite subst_ctx_distr_cons.
+      repeat rewrite subst_open_var_assoc; auto 2.
+  - apply s_forall_l with (add x L) ([e3 / x] e) k.
+    + now apply subst_mono; auto.
+    + auto.
+    + auto.
+    + rewrite <- subst_open_distr; auto.
+    + intros. distribute_ctx. rewrite subst_ctx_distr_cons.
+      repeat rewrite subst_open_var_assoc; auto 2.
+  - apply s_forall_r with (add x L) k.
+    + auto.
+    + auto.
+    + intros. distribute_ctx. rewrite subst_ctx_distr_cons.
+      repeat rewrite subst_open_var_assoc; auto 2.
+  - apply s_forall_2 with (add x L) k.
+    + auto.
+    + intros. distribute_ctx. rewrite subst_ctx_distr_cons.
+      repeat rewrite subst_open_var_assoc; auto 2.
+  - eauto.
+
+  - destruct Γ2; inversion H.
+  - destruct Γ2; inversion H1; subst; simpl in *.
+    + auto.
+    + apply wf_cons with k; auto.
+      rewrite dom_app. rewrite dom_subst_equal.
+      intro. apply in_subset with (s2 := dom (Γ1 , x0 : B ,, Γ2)) in H2.
+      contradiction.
+      apply dom_insert_subset.
+  - assumption.
+Qed.
 
 Theorem transitivity : forall e2 Γ e1 e3 A B,
   Γ ⊢ e1 <: e2 : A -> Γ ⊢ e2 <: e3 : B -> Γ ⊢ e1 <: e3 : A.
 Proof.
-  intro. assert (lc_expr e2) by admit.
-  induction H; intros Γ e1' e3' A' B' Hsubl;
-    generalize dependent e3'; generalize dependent B'.
-  - dependent induction Hsubl; intros B' e3' Hsubr.
-    + dependent induction Hsubr.
-      * auto.
-      * assert ( binds x * G ) by now apply var_star_inversion.
-        apply binds_inversion in H0.
-        destruct H0 as [Γ1 [Γ2 E]].
-        rewrite E in H3, H.
-        assert ( * = A ) by (eapply binds_type_equal; eassumption).
-        rewrite <- H0 in *. apply s_forall_r with L k; eauto.
-      * eauto 3.
-    + eauto.
-    + eauto.
-  - dependent induction Hsubl; intros B' e3' Hsubr.
-    + dependent induction Hsubr.
-      * auto.
-      * apply star_type_inversion in Hsubr2. inversion Hsubr2.
-      * apply IHHsubr1; auto.
-    + eauto.
-    + eauto.
-  - dependent induction Hsubl; intros B' e3' Hsubr.
-    + dependent induction Hsubr.
-      * eauto 3.
-      * apply num_not_of_star in Hsubr2. contradiction.
-      * eauto 3.
-    + eauto 3.
-    + eauto 3.
-  - dependent induction Hsubl; intros B' e3' Hsubr.
-    + dependent induction Hsubr; eauto 3.
-    + eauto 3.
-    + eauto 3.
-  - dependent induction Hsubl; intros B' e3' Hsubr.
-    + dependent induction Hsubr.
-      * eauto 3.
-      * admit.
-      * eauto 3.
-    + eauto 3.
-    + eauto 3.
-  - dependent induction Hsubl; intros B' e3' Hsubr.
-    + dependent induction Hsubr.
-      * apply s_abs with (L `union` L1 `union` L0); eauto 1.
-        intros. apply H1 with x (B0 <^> x); auto 2.
-      * apply abs_not_of_star in Hsubr2. contradiction.
-      * eauto 2.
-    + eauto 3.
-    + eauto 3.
-  - dependent induction Hsubl; intros B' e3' Hsubr.
-    + dependent induction Hsubr.
-      * apply s_pi with (L `union` L0 `union` L1) k3; admit.
-      * admit.
-      * eauto 2.
-    + eauto 3.
-    + eauto 3.
-  - dependent induction Hsubl; intros B' e3' Hsubr.
-    + eauto 3.
-    + admit.
-    + admit.
-    + eauto 3.
-  - dependent induction Hsubl; intros B' e3' Hsubr.
-    + dependent induction Hsubr.
-      * apply s_forall with (L `union` L0 `union` L1) k; eauto 3.
-        intros. eapply H1. eauto. auto. apply H5. auto.
-      * apply bind_not_of_star in Hsubr2. contradiction.
-      * eauto 2.
-    + eauto 3.
-    + eauto 3.
-Admitted.
-
-Theorem transitivity' : forall e2 Γ e1 e3 A,
-  Γ ⊢ e1 <: e2 : A -> Γ ⊢ e2 <: e3 : A -> Γ ⊢ e1 <: e3 : A.
-Proof.
-  intro. assert (lc_expr e2) by admit.
-  induction H; intros Γ e1' e3' A' Hsubl;
-    generalize dependent e3'.
-  - dependent induction Hsubl; intros e3' Hsubr.
-    + assumption.
-    + eauto.
-    + admit.
-Admitted.
-
-Lemma binds_var_consistent : forall Γ x A B,
-    Γ ⊢ e_var_f x <: e_var_f x : A -> x : B ∈ Γ -> Γ ⊢ B <: A : *.
-Proof.
-  intros.
-  dependent induction H.
-  - induction G.
-    + inversion H0.
-    + destruct a. unfold binds in *. simpl in *.
-      destruct H0.
-      * inversion H0. subst. destruct H1; inversion H; subst.
-        ** inversion H1. subst.
-           now apply weakening_cons.
-        ** now apply binds__in_dom in H1.
-      * destruct H1; inversion H; subst.
-        ** inversion H1. subst.
-           now apply binds__in_dom in H0.
-        ** apply weakening_cons; auto.
-  - admit. (* need transitivity *)
 Admitted.
 
 Theorem type_consistency : forall Γ e1 e2 A B,
   Γ ⊢ e1 : A -> Γ ⊢ e1 <: e2 : B -> Γ ⊢ e1 <: e2 : A.
 Proof.
-  intros Γ e1 e2 A B Hsub1 Hsub.
-  generalize dependent A.
-  induction Hsub; intros.
-  - assumption.
-  - assumption.
-  - assumption.
-  - assumption.
-  - generalize dependent L.
-    dependent induction Hsub1; intros.
-    + apply s_abs with (L `union` L0).
-      * assumption.
-      * intros.
-        apply H2. auto.
-        apply H. auto.
-    + apply s_sub with A0.
-      * apply IHHsub1_1 with L; auto.
-      * assumption.
-  - dependent induction Hsub0.
-    + apply s_pi with (L `union` L0); auto.
-    + apply s_sub with A.
-      * apply IHHsub0_1; auto.
-      * assumption.
-  - dependent induction Hsub0.
-    + apply s_app with A0.
-      * assumption.
-      * apply IHHsub2. assumption.
-    + apply s_sub with A0.
-      * apply IHHsub0_1; auto.
-      * assumption.
-  - dependent induction Hsub1.
-    + apply s_forall with (L0 `union` L).
-      * assumption.
-      * assumption.
-      * intros. apply H1; auto.
-    + apply s_sub with A0; auto.
-  - dependent induction Hsub0.
-    + apply s_forall_l with L e; assumption.
-    + apply s_forall_l with L e; assumption.
-    + apply s_forall_l with L e; assumption.
-    + apply s_sub with A0.
-      * apply IHHsub0_1; auto.
-      * assumption.
-  - dependent induction Hsub0; eauto 3.
-    + admit.
-    + admit.
-    + admit.
-    + admit.
-    + admit.
-  - dependent induction Hsub1; eauto 3.
-  - auto.
 Admitted.
 
 Theorem type_correct : forall Γ A B C, Γ ⊢ A <: B : C -> Γ ⊢ C : *.
-Proof.
-Admitted.
-
-Theorem substitution : forall Γ1 Γ2 x A B e1 e2 e3,
-  Γ1 , x : B ,, Γ2 ⊢ e1 <: e2 : A ->
-  Γ1 ⊢ e3 : B ->
-  Γ1 ,, subst_context x e3 Γ2 ⊢
-    subst_expr e3 x e1 <: subst_expr e3 x e2 : subst_expr e3 x A.
 Proof.
 Admitted.
